library/init/data/rbmap/basic.lean
@@ -11,62 +11,62 @@ universes u v w w'
 inductive Rbcolor
 | red | black
 
-inductive Rbnode (α : Type u) (β : α → Type v)
-| leaf  {}                                                                            : Rbnode
-| Node  (color : Rbcolor) (lchild : Rbnode) (key : α) (val : β key) (rchild : Rbnode) : Rbnode
+inductive RBNode (α : Type u) (β : α → Type v)
+| leaf  {}                                                                            : RBNode
+| Node  (color : Rbcolor) (lchild : RBNode) (key : α) (val : β key) (rchild : RBNode) : RBNode
 
-namespace Rbnode
+namespace RBNode
 variables {α : Type u} {β : α → Type v} {σ : Type w}
 
 open Rbcolor Nat
 
-def depth (f : Nat → Nat → Nat) : Rbnode α β → Nat
+def depth (f : Nat → Nat → Nat) : RBNode α β → Nat
 | leaf               := 0
 | (Node _ l _ _ r)   := succ (f (depth l) (depth r))
 
-protected def min : Rbnode α β → Option (Σ k : α, β k)
+protected def min : RBNode α β → Option (Σ k : α, β k)
 | leaf                  := none
 | (Node _ leaf k v _)   := some ⟨k, v⟩
 | (Node _ l k v _)      := min l
 
-protected def max : Rbnode α β → Option (Σ k : α, β k)
+protected def max : RBNode α β → Option (Σ k : α, β k)
 | leaf                  := none
 | (Node _ _ k v leaf)   := some ⟨k, v⟩
 | (Node _ _ k v r)      := max r
 
-@[specialize] def fold (f : Π (k : α), β k → σ → σ) : Rbnode α β → σ → σ
+@[specialize] def fold (f : Π (k : α), β k → σ → σ) : RBNode α β → σ → σ
 | leaf b               := b
 | (Node _ l k v r)   b := fold r (f k v (fold l b))
 
-@[specialize] def mfold {m : Type w → Type w'} [Monad m] (f : Π (k : α), β k → σ → m σ) : Rbnode α β → σ → m σ
+@[specialize] def mfold {m : Type w → Type w'} [Monad m] (f : Π (k : α), β k → σ → m σ) : RBNode α β → σ → m σ
 | leaf b               := pure b
 | (Node _ l k v r) b   := do b₁ ← mfold l b, b₂ ← f k v b₁, mfold r b₂
 
-@[specialize] def revFold (f : Π (k : α), β k → σ → σ) : Rbnode α β → σ → σ
+@[specialize] def revFold (f : Π (k : α), β k → σ → σ) : RBNode α β → σ → σ
 | leaf b               := b
 | (Node _ l k v r)   b := revFold l (f k v (revFold r b))
 
-@[specialize] def all (p : Π k : α, β k → Bool) : Rbnode α β → Bool
+@[specialize] def all (p : Π k : α, β k → Bool) : RBNode α β → Bool
 | leaf                 := true
 | (Node _ l k v r)     := p k v && all l && all r
 
-@[specialize] def any (p : Π k : α, β k → Bool) : Rbnode α β → Bool
+@[specialize] def any (p : Π k : α, β k → Bool) : RBNode α β → Bool
 | leaf                 := false
 | (Node _ l k v r)   := p k v || any l || any r
 
-def balance1 : Rbnode α β → Rbnode α β → Rbnode α β
+def balance1 : RBNode α β → RBNode α β → RBNode α β
 | (Node _ _ kv vv t) (Node _ (Node red l kx vx r₁) ky vy r₂) := Node red (Node black l kx vx r₁) ky vy (Node black r₂ kv vv t)
 | (Node _ _ kv vv t) (Node _ l₁ ky vy (Node red l₂ kx vx r)) := Node red (Node black l₁ ky vy l₂) kx vx (Node black r kv vv t)
 | (Node _ _ kv vv t) (Node _ l  ky vy r)                     := Node black (Node red l ky vy r) kv vv t
 | _                                                        _ := leaf -- unreachable
 
-def balance2 : Rbnode α β → Rbnode α β → Rbnode α β
+def balance2 : RBNode α β → RBNode α β → RBNode α β
 | (Node _ t kv vv _) (Node _ (Node red l kx₁ vx₁ r₁) ky vy r₂)  := Node red (Node black t kv vv l) kx₁ vx₁ (Node black r₁ ky vy r₂)
 | (Node _ t kv vv _) (Node _ l₁ ky vy (Node red l₂ kx₂ vx₂ r₂)) := Node red (Node black t kv vv l₁) ky vy (Node black l₂ kx₂ vx₂ r₂)
 | (Node _ t kv vv _) (Node _ l ky vy r)                         := Node black t kv vv (Node red l ky vy r)
 | _                                                        _    := leaf -- unreachable
 
-def isRed : Rbnode α β → Bool
+def isRed : RBNode α β → Bool
 | (Node red _ _ _ _) := true
 | _                  := false
 
@@ -74,7 +74,7 @@ section insert
 
 variables (lt : α → α → Prop) [DecidableRel lt]
 
-def ins : Rbnode α β → Π k : α, β k → Rbnode α β
+def ins : RBNode α β → Π k : α, β k → RBNode α β
 | leaf                 kx vx := Node red leaf kx vx leaf
 | (Node red a ky vy b) kx vx :=
    (match cmpUsing lt kx ky with
@@ -91,11 +91,11 @@ def ins : Rbnode α β → Π k : α, β k → Rbnode α β
       if isRed b then balance2 (Node black a ky vy leaf) (ins b kx vx)
       else Node black a ky vy (ins b kx vx)
 
-def setBlack : Rbnode α β → Rbnode α β
+def setBlack : RBNode α β → RBNode α β
 | (Node _ l k v r) := Node black l k v r
 | e                := e
 
-def insert (t : Rbnode α β) (k : α) (v : β k) : Rbnode α β :=
+def insert (t : RBNode α β) (k : α) (v : β k) : RBNode α β :=
 if isRed t then setBlack (ins lt t k v)
 else ins lt t k v
 
@@ -106,7 +106,7 @@ variable (lt : α → α → Prop)
 
 variable [DecidableRel lt]
 
-def findCore : Rbnode α β → Π k : α, Option (Σ k : α, β k)
+def findCore : RBNode α β → Π k : α, Option (Σ k : α, β k)
 | leaf               x := none
 | (Node _ a ky vy b) x :=
   (match cmpUsing lt x ky with
@@ -114,7 +114,7 @@ def findCore : Rbnode α β → Π k : α, Option (Σ k : α, β k)
    | Ordering.Eq := some ⟨ky, vy⟩
    | Ordering.gt := findCore b x)
 
-def find {β : Type v} : Rbnode α (λ _, β) → α → Option β
+def find {β : Type v} : RBNode α (λ _, β) → α → Option β
 | leaf                 x := none
 | (Node _ a ky vy b) x :=
   (match cmpUsing lt x ky with
@@ -122,7 +122,7 @@ def find {β : Type v} : Rbnode α (λ _, β) → α → Option β
    | Ordering.Eq := some vy
    | Ordering.gt := find b x)
 
-def lowerBound : Rbnode α β → α → Option (Sigma β) → Option (Sigma β)
+def lowerBound : RBNode α β → α → Option (Sigma β) → Option (Sigma β)
 | leaf               x lb := lb
 | (Node _ a ky vy b) x lb :=
   (match cmpUsing lt x ky with
@@ -132,95 +132,95 @@ def lowerBound : Rbnode α β → α → Option (Sigma β) → Option (Sigma β)
 
 end membership
 
-inductive WellFormed (lt : α → α → Prop) : Rbnode α β → Prop
+inductive WellFormed (lt : α → α → Prop) : RBNode α β → Prop
 | leafWff : WellFormed leaf
-| insertWff {n n' : Rbnode α β} {k : α} {v : β k} [DecidableRel lt] : WellFormed n → n' = insert lt n k v → WellFormed n'
+| insertWff {n n' : RBNode α β} {k : α} {v : β k} [DecidableRel lt] : WellFormed n → n' = insert lt n k v → WellFormed n'
 
-end Rbnode
+end RBNode
 
-open Rbnode
+open RBNode
 
-/- TODO(Leo): define dRbmap -/
+/- TODO(Leo): define dRBMap -/
 
-def Rbmap (α : Type u) (β : Type v) (lt : α → α → Prop) : Type (max u v) :=
-{t : Rbnode α (λ _, β) // t.WellFormed lt }
+def RBMap (α : Type u) (β : Type v) (lt : α → α → Prop) : Type (max u v) :=
+{t : RBNode α (λ _, β) // t.WellFormed lt }
 
-@[inline] def mkRbmap (α : Type u) (β : Type v) (lt : α → α → Prop) : Rbmap α β lt :=
+@[inline] def mkRBMap (α : Type u) (β : Type v) (lt : α → α → Prop) : RBMap α β lt :=
 ⟨leaf, WellFormed.leafWff lt⟩
 
-namespace Rbmap
+namespace RBMap
 variables {α : Type u} {β : Type v} {σ : Type w} {lt : α → α → Prop}
 
-def depth (f : Nat → Nat → Nat) (t : Rbmap α β lt) : Nat :=
+def depth (f : Nat → Nat → Nat) (t : RBMap α β lt) : Nat :=
 t.val.depth f
 
-@[inline] def fold (f : α → β → σ → σ) : Rbmap α β lt → σ → σ
+@[inline] def fold (f : α → β → σ → σ) : RBMap α β lt → σ → σ
 | ⟨t, _⟩ b := t.fold f b
 
-@[inline] def revFold (f : α → β → σ → σ) : Rbmap α β lt → σ → σ
+@[inline] def revFold (f : α → β → σ → σ) : RBMap α β lt → σ → σ
 | ⟨t, _⟩ b := t.revFold f b
 
-@[inline] def mfold {m : Type w → Type w'} [Monad m] (f : α → β → σ → m σ) : Rbmap α β lt → σ → m σ
+@[inline] def mfold {m : Type w → Type w'} [Monad m] (f : α → β → σ → m σ) : RBMap α β lt → σ → m σ
 | ⟨t, _⟩ b := t.mfold f b
 
-@[inline] def mfor {m : Type w → Type w'} [Monad m] (f : α → β → m σ) (t : Rbmap α β lt) : m Punit :=
+@[inline] def mfor {m : Type w → Type w'} [Monad m] (f : α → β → m σ) (t : RBMap α β lt) : m PUnit :=
 t.mfold (λ k v _, f k v *> pure ⟨⟩) ⟨⟩
 
-@[inline] def Empty : Rbmap α β lt → Bool
+@[inline] def Empty : RBMap α β lt → Bool
 | ⟨leaf, _⟩ := true
 | _         := false
 
-@[specialize] def toList : Rbmap α β lt → List (α × β)
+@[specialize] def toList : RBMap α β lt → List (α × β)
 | ⟨t, _⟩ := t.revFold (λ k v ps, (k, v)::ps) []
 
-@[inline] protected def min : Rbmap α β lt → Option (α × β)
+@[inline] protected def min : RBMap α β lt → Option (α × β)
 | ⟨t, _⟩ :=
   match t.min with
   | some ⟨k, v⟩ := some (k, v)
   | none        := none
 
-@[inline] protected def max : Rbmap α β lt → Option (α × β)
+@[inline] protected def max : RBMap α β lt → Option (α × β)
 | ⟨t, _⟩ :=
   match t.max with
   | some ⟨k, v⟩ := some (k, v)
   | none        := none
 
-instance [HasRepr α] [HasRepr β] : HasRepr (Rbmap α β lt) :=
+instance [HasRepr α] [HasRepr β] : HasRepr (RBMap α β lt) :=
 ⟨λ t, "rbmapOf " ++ repr t.toList⟩
 
 variables [DecidableRel lt]
 
-def insert : Rbmap α β lt → α → β → Rbmap α β lt
+def insert : RBMap α β lt → α → β → RBMap α β lt
 | ⟨t, w⟩   k v := ⟨t.insert lt k v, WellFormed.insertWff w rfl⟩
 
-@[specialize] def ofList : List (α × β) → Rbmap α β lt
-| []          := mkRbmap _ _ _
+@[specialize] def ofList : List (α × β) → RBMap α β lt
+| []          := mkRBMap _ _ _
 | (⟨k,v⟩::xs) := (ofList xs).insert k v
 
-def findCore : Rbmap α β lt → α → Option (Σ k : α, β)
+def findCore : RBMap α β lt → α → Option (Σ k : α, β)
 | ⟨t, _⟩ x := t.findCore lt x
 
-def find : Rbmap α β lt → α → Option β
+def find : RBMap α β lt → α → Option β
 | ⟨t, _⟩ x := t.find lt x
 
 /-- (lowerBound k) retrieves the kv pair of the largest key smaller than or equal to `k`,
     if it exists. -/
-def lowerBound : Rbmap α β lt → α → Option (Σ k : α, β)
+def lowerBound : RBMap α β lt → α → Option (Σ k : α, β)
 | ⟨t, _⟩ x := t.lowerBound lt x none
 
-@[inline] def contains (t : Rbmap α β lt) (a : α) : Bool :=
+@[inline] def contains (t : RBMap α β lt) (a : α) : Bool :=
 (t.find a).isSome
 
-def fromList (l : List (α × β)) (lt : α → α → Prop) [DecidableRel lt] : Rbmap α β lt :=
-l.foldl (λ r p, r.insert p.1 p.2) (mkRbmap α β lt)
+def fromList (l : List (α × β)) (lt : α → α → Prop) [DecidableRel lt] : RBMap α β lt :=
+l.foldl (λ r p, r.insert p.1 p.2) (mkRBMap α β lt)
 
-@[inline] def all : Rbmap α β lt → (α → β → Bool) → Bool
+@[inline] def all : RBMap α β lt → (α → β → Bool) → Bool
 | ⟨t, _⟩ p := t.all p
 
-@[inline] def any : Rbmap α β lt → (α → β → Bool) → Bool
+@[inline] def any : RBMap α β lt → (α → β → Bool) → Bool
 | ⟨t, _⟩ p := t.any p
 
-end Rbmap
+end RBMap
 
-def rbmapOf {α : Type u} {β : Type v} (l : List (α × β)) (lt : α → α → Prop) [DecidableRel lt] : Rbmap α β lt :=
-Rbmap.fromList l lt
+def rbmapOf {α : Type u} {β : Type v} (l : List (α × β)) (lt : α → α → Prop) [DecidableRel lt] : RBMap α β lt :=
+RBMap.fromList l lt
