library/init/data/rbtree/basic.lean
@@ -7,82 +7,82 @@ prelude
 import init.data.rbmap.basic
 universes u v w
 
-def Rbtree (α : Type u) (lt : α → α → Prop) : Type u :=
-Rbmap α Unit lt
+def RBTree (α : Type u) (lt : α → α → Prop) : Type u :=
+RBMap α Unit lt
 
-@[inline] def mkRbtree (α : Type u) (lt : α → α → Prop) : Rbtree α lt :=
-mkRbmap α Unit lt
+@[inline] def mkRBTree (α : Type u) (lt : α → α → Prop) : RBTree α lt :=
+mkRBMap α Unit lt
 
-namespace Rbtree
+namespace RBTree
 variables {α : Type u} {β : Type v} {lt : α → α → Prop}
 
-@[inline] def depth (f : Nat → Nat → Nat) (t : Rbtree α lt) : Nat :=
-Rbmap.depth f t
+@[inline] def depth (f : Nat → Nat → Nat) (t : RBTree α lt) : Nat :=
+RBMap.depth f t
 
-@[inline] def fold (f : α → β → β) (t : Rbtree α lt) (b : β) : β :=
-Rbmap.fold (λ a _ r, f a r) t b
+@[inline] def fold (f : α → β → β) (t : RBTree α lt) (b : β) : β :=
+RBMap.fold (λ a _ r, f a r) t b
 
-@[inline] def revFold (f : α → β → β) (t : Rbtree α lt) (b : β) : β :=
-Rbmap.revFold (λ a _ r, f a r) t b
+@[inline] def revFold (f : α → β → β) (t : RBTree α lt) (b : β) : β :=
+RBMap.revFold (λ a _ r, f a r) t b
 
-@[inline] def mfold {m : Type v → Type w} [Monad m] (f : α → β → m β) (t : Rbtree α lt) (b : β) : m β :=
-Rbmap.mfold (λ a _ r, f a r) t b
+@[inline] def mfold {m : Type v → Type w} [Monad m] (f : α → β → m β) (t : RBTree α lt) (b : β) : m β :=
+RBMap.mfold (λ a _ r, f a r) t b
 
-@[inline] def mfor {m : Type v → Type w} [Monad m] (f : α → m β) (t : Rbtree α lt) : m Punit :=
+@[inline] def mfor {m : Type v → Type w} [Monad m] (f : α → m β) (t : RBTree α lt) : m PUnit :=
 t.mfold (λ a _, f a *> pure ⟨⟩) ⟨⟩
 
-@[inline] def Empty (t : Rbtree α lt) : Bool :=
-Rbmap.Empty t
+@[inline] def Empty (t : RBTree α lt) : Bool :=
+RBMap.Empty t
 
-@[specialize] def toList (t : Rbtree α lt) : List α :=
+@[specialize] def toList (t : RBTree α lt) : List α :=
 t.revFold (::) []
 
-@[inline] protected def min (t : Rbtree α lt) : Option α :=
-match Rbmap.min t with
+@[inline] protected def min (t : RBTree α lt) : Option α :=
+match RBMap.min t with
 | some ⟨a, _⟩ := some a
 | none        := none
 
-@[inline] protected def max (t : Rbtree α lt) : Option α :=
-match Rbmap.max t with
+@[inline] protected def max (t : RBTree α lt) : Option α :=
+match RBMap.max t with
 | some ⟨a, _⟩ := some a
 | none        := none
 
-instance [HasRepr α] : HasRepr (Rbtree α lt) :=
+instance [HasRepr α] : HasRepr (RBTree α lt) :=
 ⟨λ t, "rbtreeOf " ++ repr t.toList⟩
 
 variables [DecidableRel lt]
 
-@[inline] def insert (t : Rbtree α lt) (a : α) : Rbtree α lt :=
-Rbmap.insert t a ()
+@[inline] def insert (t : RBTree α lt) (a : α) : RBTree α lt :=
+RBMap.insert t a ()
 
-@[specialize] def ofList : List α → Rbtree α lt
-| []      := mkRbtree _ _
+@[specialize] def ofList : List α → RBTree α lt
+| []      := mkRBTree _ _
 | (x::xs) := (ofList xs).insert x
 
-def find (t : Rbtree α lt) (a : α) : Option α :=
-match Rbmap.findCore t a with
+def find (t : RBTree α lt) (a : α) : Option α :=
+match RBMap.findCore t a with
 | some ⟨a, _⟩ := some a
 | none        := none
 
-@[inline] def contains (t : Rbtree α lt) (a : α) : Bool :=
+@[inline] def contains (t : RBTree α lt) (a : α) : Bool :=
 (t.find a).isSome
 
-def fromList (l : List α) (lt : α → α → Prop) [DecidableRel lt] : Rbtree α lt :=
-l.foldl insert (mkRbtree α lt)
+def fromList (l : List α) (lt : α → α → Prop) [DecidableRel lt] : RBTree α lt :=
+l.foldl insert (mkRBTree α lt)
 
-@[inline] def all (t : Rbtree α lt) (p : α → Bool) : Bool :=
-Rbmap.all t (λ a _, p a)
+@[inline] def all (t : RBTree α lt) (p : α → Bool) : Bool :=
+RBMap.all t (λ a _, p a)
 
-@[inline] def any (t : Rbtree α lt) (p : α → Bool) : Bool :=
-Rbmap.any t (λ a _, p a)
+@[inline] def any (t : RBTree α lt) (p : α → Bool) : Bool :=
+RBMap.any t (λ a _, p a)
 
-def subset (t₁ t₂ : Rbtree α lt) : Bool :=
+def subset (t₁ t₂ : RBTree α lt) : Bool :=
 t₁.all $ λ a, (t₂.find a).toBool
 
-def seteq (t₁ t₂ : Rbtree α lt) : Bool :=
+def seteq (t₁ t₂ : RBTree α lt) : Bool :=
 subset t₁ t₂ && subset t₂ t₁
 
-end Rbtree
+end RBTree
 
-def rbtreeOf {α : Type u} (l : List α) (lt : α → α → Prop) [DecidableRel lt] : Rbtree α lt :=
-Rbtree.fromList l lt
+def rbtreeOf {α : Type u} (l : List α) (lt : α → α → Prop) [DecidableRel lt] : RBTree α lt :=
+RBTree.fromList l lt
