library/init/lean/parser/trie.lean
@@ -13,19 +13,19 @@ namespace Lean
 namespace Parser
 
 inductive Trie (α : Type)
-| Node : Option α → Rbnode Char (λ _, Trie) → Trie
+| Node : Option α → RBNode Char (λ _, Trie) → Trie
 
 namespace Trie
 variables {α : Type}
 
 protected def mk : Trie α :=
-⟨none, Rbnode.leaf⟩
+⟨none, RBNode.leaf⟩
 
 private def insertAux (val : α) : Nat → Trie α → String.Iterator → Trie α
 | 0     (Trie.Node _ map)    _ := Trie.Node (some val) map   -- NOTE: overrides old value
 | (n+1) (Trie.Node val map) it :=
-  let t' := (Rbnode.find (<) map it.curr).getOrElse Trie.mk in
-  Trie.Node val (Rbnode.insert (<) map it.curr (insertAux n t' it.next))
+  let t' := (RBNode.find (<) map it.curr).getOrElse Trie.mk in
+  Trie.Node val (RBNode.insert (<) map it.curr (insertAux n t' it.next))
 
 def insert (t : Trie α) (s : String) (val : α) : Trie α :=
 insertAux val s.length t s.mkIterator
@@ -33,7 +33,7 @@ insertAux val s.length t s.mkIterator
 private def findAux : Nat → Trie α → String.Iterator → Option α
 | 0     (Trie.Node val _)    _ := val
 | (n+1) (Trie.Node val map) it := do
-  t' ← Rbnode.find (<) map it.curr,
+  t' ← RBNode.find (<) map it.curr,
   findAux n t' it.next
 
 def find (t : Trie α) (s : String) : Option α :=
@@ -43,7 +43,7 @@ private def matchPrefixAux : Nat → Trie α → String.Iterator → Option (Str
 | 0     (Trie.Node val map) it Acc := Prod.mk it <$> val <|> Acc
 | (n+1) (Trie.Node val map) it Acc :=
   let Acc' := Prod.mk it <$> val <|> Acc in
-  match Rbnode.find (<) map it.curr with
+  match RBNode.find (<) map it.curr with
     | some t := matchPrefixAux n t it.next Acc'
     | none   := Acc'
 
@@ -51,7 +51,7 @@ def matchPrefix {α : Type} (t : Trie α) (it : String.Iterator) : Option (Strin
 matchPrefixAux it.remaining t it none
 
 private def toStringAux {α : Type} : Trie α → List Format
-| (Trie.Node val map) := flip Rbnode.fold map (λ c t Fs,
+| (Trie.Node val map) := flip RBNode.fold map (λ c t Fs,
   toFormat (repr c) :: (Format.group $ Format.nest 2 $ flip Format.joinSep Format.line $ toStringAux t) :: Fs) []
 
 instance {α : Type} : HasToString (Trie α) :=
